\begin{itemize}
	\item $\left(a + b\right) \;\%\; c = 
	      \left(\left(a \;\%\; c\right) + 
	      \left(b \;\%\; c\right)\right) \;\%\; c$
	\item $\left(a - b\right) \;\%\; c = 
	      \left(\left[\left(a \;\%\; c\right) -
	      \left(b \;\%\; c\right)\right] + c\right) \;\%\; c$
	\item $\left(a \times b\right) \;\%\; c = 
	      \left(\left(a \;\%\; c\right) \times
	      \left(b \;\%\; c\right)\right) \;\%\; c$
	\item $\left(a \div b\right) \;\%\; c = 
	      \left(\left(a \;\%\; c\right) \times
	      \left(b^{-1} \;\%\; c\right)\right) \;\%\; c$
	\item $a^{b} \;\%\; c = \left(a \;\%\; c\right)^{b} \;\%\; c$
\end{itemize}

\begin{lstlisting}[language=C++, title=ExponenciaÃ§Ã£o Modular]
int fastPower(int x, int n, int MOD) {
    int y = x, result = 1;
    while (n > 0) {
        if (n & 1) result = (result % MOD * y % MOD) % MOD;
        y = (y % MOD * y % MOD) % MOD;
        n >>= 1;
    }
    return result;
}
\end{lstlisting}
